Clean/Gadgets/Keccak/ThetaXor.lean
@@ -15,16 +15,9 @@ def main : Var Inputs (F p) → Circuit (F p) (Var KeccakState (F p))
   | { state, d } => .mapFinRange 25 fun i =>
     Xor64.circuit ⟨state[i.val], d[i.val / 5]⟩
 
--- TODO AUTOELAB fails probably bc of match
 @[reducible]
-instance elaborated : ElaboratedCircuit (F p) Inputs KeccakState main where
-  localLength _ := 200
-  output _ i₀ := .mapFinRange 25 fun i => varFromOffset U64 (i₀ + i.val * 8)
-
-  localLength_eq _ n := by simp only [main, circuit_norm, Xor64.circuit, Xor64.elaborated]
-  output_eq _ i := by simp only [main, circuit_norm, Xor64.circuit, Xor64.elaborated]
-  subcircuitsConsistent _ i := by simp only [main, circuit_norm]
-  channelsLawful := by simp only [main, circuit_norm, Xor64.circuit, Xor64.elaborated]
+instance elaborated : ElaboratedCircuit (F p) Inputs KeccakState main := by
+  infer_elaborated_circuit_reduced
 
 def Assumptions (inputs : Inputs (F p)) : Prop :=
   let ⟨state, d⟩ := inputs
